coq/extracted/Extract.v
@@ -21,7 +21,7 @@ Extraction Blacklist String List Char Core Monad Bool Vector Format Nat Int Opti
 (* Debugging print *)
 Extraction NoInline Common.Utils.print_msg.
 Extract Constant Common.Utils.print_msg => "print_endline".
-Extract Inlined Constant Morello.Capability.strfcap => "strfcap".
+Extract Inlined Constant Morello.Capability_GS.strfcap => "strfcap".
 
 (* Used by Coq's Real library *)
 Extract Constant ClassicalDedekindReals.sig_forall_dec => "fun _ -> assert false".
